src/impl/TLS13.Impl.Handle.ChangeCipherSpec.fsti
@@ -32,13 +32,21 @@ fn handle_change_cipher_spec
            B.length 'old_app_out == SZ.v app_out_len /\
            L.tls_message_is_change_cipher_spec l)
   returns resp: CT.client_response
-  ensures exists* st1 m network_out_bytes app_out_bytes.
-          C.connection_exactly c st1 **
+  ensures C.connection_exactly c (C.local_fail_state 'st0 C.tls_unexpected_message_error) **
           pts_to raw 'raw_bytes **
-          pts_to network_out network_out_bytes **
-          pts_to app_out app_out_bytes **
-          pure (B.length network_out_bytes == SZ.v network_out_len /\
-                B.length app_out_bytes == SZ.v app_out_len /\
-                CT.legal_handled_tls_response
-                  'st0 st1 resp m (Ghost.reveal 'raw_bytes) network_out_bytes app_out_bytes /\
-                CT.some_legal_response 'st0 st1 resp network_out_bytes app_out_bytes)
+          pts_to network_out 'old_network_out **
+          pts_to app_out 'old_app_out **
+          pure (B.length 'old_network_out == SZ.v network_out_len /\
+                B.length 'old_app_out == SZ.v app_out_len /\
+                CT.unexpected_message_response
+                  'st0
+                  (C.local_fail_state 'st0 C.tls_unexpected_message_error)
+                  resp
+                  'old_network_out
+                  'old_app_out /\
+                CT.some_legal_response
+                  'st0
+                  (C.local_fail_state 'st0 C.tls_unexpected_message_error)
+                  resp
+                  'old_network_out
+                  'old_app_out)
